Examples/IMP/Analysis/Generic.lean
@@ -2,3 +2,4 @@ import Examples.IMP.Analysis.Generic.Domain
 import Examples.IMP.Analysis.Generic.Defs
 import Examples.IMP.Analysis.Generic.Lemmas
 import Examples.IMP.Analysis.Generic.Soundness
+import Examples.IMP.Analysis.Generic.Collecting
